fix(library/tactic): fixes #1513
Implement rename tactic in Lean using revert/intro

src/library/tactic/init_module.cpp
@@ -8,7 +8,6 @@ Author: Leonardo de Moura
 #include "library/tactic/tactic_state.h"
 #include "library/tactic/intro_tactic.h"
 #include "library/tactic/revert_tactic.h"
-#include "library/tactic/rename_tactic.h"
 #include "library/tactic/clear_tactic.h"
 #include "library/tactic/app_builder_tactics.h"
 #include "library/tactic/subst_tactic.h"
@@ -44,7 +43,6 @@ void initialize_tactic_module() {
     initialize_tactic_state();
     initialize_intro_tactic();
     initialize_revert_tactic();
-    initialize_rename_tactic();
     initialize_clear_tactic();
     initialize_app_builder_tactics();
     initialize_subst_tactic();
@@ -103,7 +101,6 @@ void finalize_tactic_module() {
     finalize_subst_tactic();
     finalize_app_builder_tactics();
     finalize_clear_tactic();
-    finalize_rename_tactic();
     finalize_revert_tactic();
     finalize_intro_tactic();
     finalize_tactic_state();
