tests/lean/1513.lean
@@ -1,0 +1,8 @@
+example (n : ℕ) (h : n = 0) : n = 0 :=
+by rename n m
+
+example (n : ℕ) : let x := 10 in n > 0 → x > 5 → n ≠ x → x + 1 = 1 + x :=
+begin
+  intros,
+  rename x y
+end
